

# Ackermann's function

`ackermann 0 n = n + 1`

`ackermann (m + 1) 0 = ackermann m 1`

`ackermann (m + 1) (n + 1) = ackermann m (ackermann (m + 1) n)`

# Ackermann's function

```
ackermann 0 n = n + 1
ackermann (m + 1) 0 = ackermann m 1
ackermann (m + 1) (n + 1) = ackermann m (ackermann (m + 1) n)
iterate f 0 = \x -> x
iterate f (n + 1) = \x -> f (iterate f n x)
```

# Ackermann's function

```
ackermann 0 n = n + 1
ackermann (m + 1) 0 = ackermann m 1
ackermann (m + 1) (n + 1) = ackermann m (ackermann (m + 1) n)
iterate f 0 = \x -> x
iterate f (n + 1) = \x -> f (iterate f n x)
```

## Theorem

```
ackermann (m + 1) n = iterate (ackermann m) (n + 1) 1
```

# Ackermann's function

```
ackermann 0 n = n + 1
ackermann (m + 1) 0 = ackermann m 1
ackermann (m + 1) (n + 1) = ackermann m (ackermann (m + 1) n)
iterate f 0 = \x -> x
iterate f (n + 1) = \x -> f (iterate f n x)
```

## Theorem

```
ackermann (m + 1) n = iterate (ackermann m) (n + 1) 1
```

## Proof.

By

# Ackermann's function

```
ackermann 0 n = n + 1
ackermann (m + 1) 0 = ackermann m 1
ackermann (m + 1) (n + 1) = ackermann m (ackermann (m + 1) n)
iterate f 0 = \x -> x
iterate f (n + 1) = \x -> f (iterate f n x)
```

## Theorem

```
ackermann (m + 1) n = iterate (ackermann m) (n + 1) 1
```

## Proof.

By induction on  $n$ .

- **Base case.** We need to show

# Ackermann's function

```
ackermann 0 n = n + 1
ackermann (m + 1) 0 = ackermann m 1
ackermann (m + 1) (n + 1) = ackermann m (ackermann (m + 1) n)
iterate f 0 = \x -> x
iterate f (n + 1) = \x -> f (iterate f n x)
```

## Theorem

```
ackermann (m + 1) n = iterate (ackermann m) (n + 1) 1
```

## Proof.

By induction on  $n$ .

- ▶ **Base case.** We need to show

```
ackermann (m + 1) 0 = iterate (ackermann m) (0 + 1) 1.
```

But this follows

# Ackermann's function

```
ackermann 0 n = n + 1
ackermann (m + 1) 0 = ackermann m 1
ackermann (m + 1) (n + 1) = ackermann m (ackermann (m + 1) n)
iterate f 0 = \x -> x
iterate f (n + 1) = \x -> f (iterate f n x)
```

## Theorem

$\text{ackermann } (m + 1) n = \text{iterate } (\text{ackermann } m) (n + 1) 1$

## Proof.

By induction on  $n$ .

► **Base case.** We need to show

$\text{ackermann } (m + 1) 0 = \text{iterate } (\text{ackermann } m) (0 + 1) 1.$

But this follows from definitions by computation.

```

ackermann 0 n = n + 1
ackermann (m + 1) 0 = ackermann m 1
ackermann (m + 1) (n + 1) = ackermann m (ackermann (m + 1) n)
iterate f 0 = \x -> x
iterate f (n + 1) = \x -> f (iterate f n x)

```

## Theorem

```

ackermann (m + 1) n = iterate (ackermann m) (n + 1) 1

```

## Proof.

**Inductive step.** We need to show



```
ackermann 0 n = n + 1
ackermann (m + 1) 0 = ackermann m 1
ackermann (m + 1) (n + 1) = ackermann m (ackermann (m + 1) n)
iterate f 0 = \x -> x
iterate f (n + 1) = \x -> f (iterate f n x)
```

## Theorem

```
ackermann (m + 1) n = iterate (ackermann m) (n + 1) 1
```

## Proof.

**Inductive step.** We need to show (\*):

```
ackermann (m + 1) (n + 1) = iterate (ackermann m) (n + 2) 1.
```

```

ackermann 0 n = n + 1
ackermann (m + 1) 0 = ackermann m 1
ackermann (m + 1) (n + 1) = ackermann m (ackermann (m + 1) n)
iterate f 0 = \x -> x
iterate f (n + 1) = \x -> f (iterate f n x)

```

## Theorem

```
ackermann (m + 1) n = iterate (ackermann m) (n + 1) 1
```

## Proof.

**Inductive step.** We need to show (\*):

```
ackermann (m + 1) (n + 1) = iterate (ackermann m) (n + 2) 1.
```

The induction hypothesis is

```

ackermann 0 n = n + 1
ackermann (m + 1) 0 = ackermann m 1
ackermann (m + 1) (n + 1) = ackermann m (ackermann (m + 1) n)
iterate f 0 = \x -> x
iterate f (n + 1) = \x -> f (iterate f n x)

```

## Theorem

```

ackermann (m + 1) n = iterate (ackermann m) (n + 1) 1

```

## Proof.

**Inductive step.** We need to show (\*):

```

ackermann (m + 1) (n + 1) = iterate (ackermann m) (n + 2) 1.

```

The induction hypothesis is

```

ackermann (m + 1) n = iterate (ackermann m) (n + 1) 1.

```

```

ackermann 0 n = n + 1
ackermann (m + 1) 0 = ackermann m 1
ackermann (m + 1) (n + 1) = ackermann m (ackermann (m + 1) n)
iterate f 0 = \x -> x
iterate f (n + 1) = \x -> f (iterate f n x)

```

## Theorem

```

ackermann (m + 1) n = iterate (ackermann m) (n + 1) 1

```

## Proof.

**Inductive step.** We need to show (\*):

```

ackermann (m + 1) (n + 1) = iterate (ackermann m) (n + 2) 1.

```

The induction hypothesis is

```

ackermann (m + 1) n = iterate (ackermann m) (n + 1) 1.

```

By definition we have

```

ackermann (m + 1) (n + 1) = ackermann m (ackermann (m + 1) n).

```

```

ackermann 0 n = n + 1
ackermann (m + 1) 0 = ackermann m 1
ackermann (m + 1) (n + 1) = ackermann m (ackermann (m + 1) n)
iterate f 0 = \x -> x
iterate f (n + 1) = \x -> f (iterate f n x)

```

## Theorem

```

ackermann (m + 1) n = iterate (ackermann m) (n + 1) 1

```

## Proof.

**Inductive step.** We need to show (\*):

```

ackermann (m + 1) (n + 1) = iterate (ackermann m) (n + 2) 1.

```

The induction hypothesis is

```

ackermann (m + 1) n = iterate (ackermann m) (n + 1) 1.

```

By definition we have

```

ackermann (m + 1) (n + 1) = ackermann m (ackermann (m + 1) n).

```

Now we

```

ackermann 0 n = n + 1
ackermann (m + 1) 0 = ackermann m 1
ackermann (m + 1) (n + 1) = ackermann m (ackermann (m + 1) n)
iterate f 0 = \x -> x
iterate f (n + 1) = \x -> f (iterate f n x)

```

## Theorem

```

ackermann (m + 1) n = iterate (ackermann m) (n + 1) 1

```

## Proof.

**Inductive step.** We need to show (\*):

```

ackermann (m + 1) (n + 1) = iterate (ackermann m) (n + 2) 1.

```

The induction hypothesis is

```

ackermann (m + 1) n = iterate (ackermann m) (n + 1) 1.

```

By definition we have

```

ackermann (m + 1) (n + 1) = ackermann m (ackermann (m + 1) n).

```

Now we use the inductive hypothesis, concluding:

```

ackermann (m + 1) (n + 1) =
    ackermann m (iterate (ackermann m) (n + 1) 1).

```

```

ackermann 0 n = n + 1
ackermann (m + 1) 0 = ackermann m 1
ackermann (m + 1) (n + 1) = ackermann m (ackermann (m + 1) n)
iterate f 0 = \x -> x
iterate f (n + 1) = \x -> f (iterate f n x)

```

## Theorem

```
ackermann (m + 1) n = iterate (ackermann m) (n + 1) 1
```

## Proof.

**Inductive step.** We need to show (\*):

```
ackermann (m + 1) (n + 1) = iterate (ackermann m) (n + 2) 1.
```

The induction hypothesis is

```
ackermann (m + 1) n = iterate (ackermann m) (n + 1) 1.
```

By definition we have

```
ackermann (m + 1) (n + 1) = ackermann m (ackermann (m + 1) n).
```

Now we use the inductive hypothesis, concluding:

```
ackermann (m + 1) (n + 1) =
    ackermann m (iterate (ackermann m) (n + 1) 1).
```

Then our claim (\*) follows

```

ackermann 0 n = n + 1
ackermann (m + 1) 0 = ackermann m 1
ackermann (m + 1) (n + 1) = ackermann m (ackermann (m + 1) n)
iterate f 0 = \x -> x
iterate f (n + 1) = \x -> f (iterate f n x)

```

## Theorem

```
ackermann (m + 1) n = iterate (ackermann m) (n + 1) 1
```

## Proof.

**Inductive step.** We need to show (\*):

```
ackermann (m + 1) (n + 1) = iterate (ackermann m) (n + 2) 1.
```

The induction hypothesis is

```
ackermann (m + 1) n = iterate (ackermann m) (n + 1) 1.
```

By definition we have

```
ackermann (m + 1) (n + 1) = ackermann m (ackermann (m + 1) n).
```

Now we use the inductive hypothesis, concluding:

```
ackermann (m + 1) (n + 1) =
    ackermann m (iterate (ackermann m) (n + 1) 1).
```

Then our claim (\*) follows from definitions by computation.